ImpESecureProof.v
@@ -16,6 +16,8 @@ Require Import Common.
 Require Import ImpE.
 Require Import ImpE2.
 
+Parameter g0: sec_spec.
+
 Ltac unfold_cfgs :=
   unfold ccfg_update_reg2 in *;
   unfold ccfg_to_ecfg2 in *;
@@ -44,20 +46,12 @@ Section Security.
                          | ANonEnc c => true
                          | _ => false                           
                          end).
-   (*  Definition knowledge_attack (c: com) (sl: sec_level)
-             (tobs: trace) (m0 m: mem) : Prop :=
-    forall d r' m2 k' t m',
-      merge_mem m0 m m2 ->
-      project_trace t true = tobs ->
-      cstep2 Normal d (c, reg_init2, m2, KSingle []) (r', m', k') t ->
-      tobs_sec_level sl tobs = tobs_sec_level sl (project_trace t false).
-*)
-  (* XXX need to enforce that all U are unset? *)
-  Definition knowledge_ind (m: mem) (g: sec_spec) (U: set condition)
-             (sl: sec_level) (m': mem) : Prop :=
-    forall m2 l,
+  
+  Definition knowledge_ind (m: mem) (sl: sec_level) (m': mem) : Prop :=
+    forall m2 l sl',
       merge_mem m m' m2 ->
-      sec_level_le (cur (g l) U) sl ->
+      g0 l = LevelP sl' ->
+      sec_level_le sl' sl ->
       (project_mem m2 true) l = (project_mem m2 false) l.
 
   Definition knowledge_esc (m0 m: mem) (e: esc_hatch) (m': mem) : Prop :=
@@ -72,16 +66,13 @@ Section Security.
   (* XXX This thing with e and csemantics is a little weird. Probably want to
      define one that encapsulates both, but I'm not sure how...
    *)
-  Definition secure_prog (sl: sec_level) (d: loc_mode) (g: sec_spec) (c: com) : Prop :=
+  Definition secure_prog (sl: sec_level) (d: loc_mode) (c: com) : Prop :=
     forall m0 mknown m r' m' k' t tobs,
       merge_mem m0 mknown m ->
       cstep2 Normal d (c, reg_init2, m, KSingle []) (r', m', KSingle k') t ->
       tobs = project_trace t true ->
       (exists m'' t'', tobs = Mem m'' :: t'') ->
-      (forall mind U,
-          In (Mem mind) tobs ->
-          (forall cnd, cnd_unset mind cnd <-> In cnd U) ->
-          knowledge_ind m0 g U sl mknown) ->
+      knowledge_ind m0 sl mknown ->
       (forall mdecl e,
           In (Decl e mdecl) tobs ->
           knowledge_esc m0 mdecl e mknown) ->
@@ -89,43 +80,35 @@ Section Security.
 End Security.
 
 Section Preservation.
-  (* Conditions set and unset at the beginning of execution *)
-  Parameter SC : set condition.
-  Parameter g: sec_spec.
-  Definition cnd_in_S (l: location) (m0 : mem2) : Prop :=
-    is_Cnd l /\ m0 l = VSingle (Vnat 1).
-
   Definition cterm2_ok (G: context) (d: loc_mode) (m0: mem2)
              (r: reg2) (m: mem2) (K: kill2) : Prop :=
       (forall x v1 v2 bt p,
-          (r x = VPair v1 v2 /\ (var_context G) x = Some (Typ bt p)) -> protected p SC) 
+          (r x = VPair v1 v2 /\ (var_context G) x = Some (Typ bt p)) -> protected p) 
       /\ (forall l v1 v2 bt p rt,
           (m (Not_cnd l) = VPair v1 v2 /\ (loc_context G) (Not_cnd l) = Some (Typ bt p, rt))
-          -> protected p SC)
+          -> protected p)
       /\ (forall e v md', is_esc_hatch e G ->
                           (estep2 md' d (e, reg_init2, m0, K) v ->
                            estep2 md' d (e, r, m, K) v))
       /\ project_kill K true = project_kill K false.
 
   Definition cconfig2_ok (pc: sec_policy) (md: mode) (G: context) (d: loc_mode)
-             (m0: mem2) (ccfg2: cconfig2) (G': context)
-             (K': kill2) (U: set condition): Prop :=
-    (forall i, set_In i U -> (ccfg_mem2 ccfg2) (Cnd i) = VSingle (Vnat 0))
-    /\  com_type pc md G (project_kill (ccfg_kill2 ccfg2) true) U d
+             (m0: mem2) (ccfg2: cconfig2) (G': context) (K': kill2) : Prop :=
+    com_type pc md G (project_kill (ccfg_kill2 ccfg2) true) [] d (* XXXX *)
                  (ccfg_com2 ccfg2) G' (project_kill K' true)
     /\ (forall x v1 v2 bt p,
            ((ccfg_reg2 ccfg2) x = VPair v1 v2
             /\ (var_context G) x = Some (Typ bt p))
-           -> protected p SC)
+           -> protected p)
     /\ (forall l v1 v2 bt p rt,
            ((ccfg_mem2 ccfg2) (Not_cnd l) = VPair v1 v2
             /\ (loc_context G) (Not_cnd l) = Some (Typ bt p, rt))    
-           -> protected p SC)
+           -> protected p)
     /\ (forall e v md', is_esc_hatch e G ->
                         (estep2 md' d  (e, reg_init2, m0, ccfg_kill2 ccfg2) v ->
                          estep2 md' d (e, ccfg_reg2 ccfg2, ccfg_mem2 ccfg2, ccfg_kill2 ccfg2) v))
     /\ project_kill (ccfg_kill2 ccfg2) true = project_kill (ccfg_kill2 ccfg2) false
-    /\ knowledge_ind (project_mem m0 true) g U L (project_mem m0 false).
+    /\ knowledge_ind (project_mem m0 true) L (project_mem m0 false).
 
   Lemma esc_hatch_reg_irrelevance (e : esc_hatch) :
     forall G md d r m k v r',
@@ -162,14 +145,14 @@ Section Preservation.
   (* is protected by S. This should be fine because we're assuming this for *)
   (* memories that are indistinguishable *)
   Lemma econfig2_locs_protected (e: exp) (m0: mem2):
-    forall G d r m k v v1 v2 bt bt' p p' q md md' rt e' U,
-      knowledge_ind (project_mem m0 true) g U L (project_mem m0 false) ->
+    forall G d r m k v v1 v2 bt bt' p p' q md md' rt e',
+      knowledge_ind (project_mem m0 true) L (project_mem m0 false) ->
       v = VPair v1 v2 ->
       exp_type md G d e (Typ bt p) ->
       estep2 md d (e,r,m,k) v ->
       e = Ederef e' ->
       exp_type md G d e' (Typ (Tref (Typ bt' p') md' rt) q) ->
-      protected q SC.
+      protected q.
   Proof.
   Admitted.
 
@@ -180,9 +163,9 @@ Section Preservation.
       (forall bt' (p' q: sec_policy) md' rt e',
           e = Ederef e' ->
           exp_type md G d e' (Typ (Tref (Typ bt' p') md' rt) q)
-          -> protected q SC) ->
+          -> protected q) ->
       cterm2_ok G d m0 r m k ->
-      protected p SC.
+      protected p.
   Proof.
     intros.
     remember (e,r,m,k) as ecfg.
@@ -193,29 +176,29 @@ Section Preservation.
       apply (H x v1 v2 bt p); split; auto. 
     - inversion Heqecfg; subst.
       inversion H5; subst.
-      assert (protected q SC). apply (H6 bt p0 q md' rt e); auto.
-      apply (join_protected_r SC p0 q); auto.
+      assert (protected q). apply (H6 bt p0 q md' rt e); auto.
+      apply (join_protected_r p0 q); auto.
     - destruct H2; destruct_pairs; try discriminate.
   Qed.
 
   Lemma impe2_final_config_preservation (G: context) (d: loc_mode) (m0: mem2) :
-      forall G' K' c r m k pc md r' m' t U,
+      forall G' K' c r m k pc md r' m' t,
         (forall l e v, loc_in_exp e G l -> m0 l = VSingle v) -> 
         context_wt G d ->
-        cconfig2_ok pc md G d m0 (c,r,m,k) G' K' U ->
+        cconfig2_ok pc md G d m0 (c,r,m,k) G' K' ->
         cstep2 md d (c,r,m,k) (r', m', K') t ->
         cterm2_ok G' d m0 r' m' K'.
   Proof.
-    intros G' K' c r m k pc md r' m' t U Hlocs Hcwt Hcfgok Hcstep.
+    intros G' K' c r m k pc md r' m' t Hlocs Hcwt Hcfgok Hcstep.
     remember (c,r,m,k) as ccfg2; subst.
     unfold cconfig2_ok in Hcfgok; destruct_pairs.
     induction c; unfold cterm2_ok; intros; subst; simpl in *; unfold_cfgs.
     (* CSkip *)
     - inversion Hcstep; try discriminate; subst.
-        inversion H0; try discriminate; subst.
+        inversion H; try discriminate; subst.
       split; [intros | split; intros]; simpl in *; auto.
-      -- now apply H1 in H7.
-      -- now apply H2 in H7.
+      -- now apply H0 in H6.
+      -- now apply H1 in H6.
 (*    (* CAssign *)
     - inversion H3; try discriminate; subst;
         inversion H4; try discriminate; subst.
@@ -224,9 +207,9 @@ Section Preservation.
          destruct (Nat.eq_dec x0 x).
          --- rewrite <- (Nat.eqb_eq x0 x) in e; rewrite e in H9.
              destruct_pairs.
-             assert (protected p S).
+             assert (protected p).
              apply (econfig2_pair_protected
-                      md (Cntxt vc lc) d e0 p r m' K' v0 v1 v2 S s H m0
+                      md (Cntxt vc lc) d e0 p r m' K' v0 v1 v2 s H m0
                       H9 H11 H16).
              (* XXX ergh now we either have to pass in the assumption or *)
              (* do something weird *)
@@ -234,7 +217,7 @@ Section Preservation.
              ---- unfold cterm2_ok; split; intros. now apply H5 in H13.
              ----- split; intros. now apply H6 in H13.
              ------ split; intros; auto.
-             ---- inversion H10; subst. now apply (join_protected_l S p pc).
+             ---- inversion H10; subst. now apply (join_protected_l p pc).
          --- rewrite <- (Nat.eqb_neq x0 x) in n. rewrite n in H9.
              apply H5 in H9; auto.
       -- now apply H6 in H9.
@@ -257,17 +240,16 @@ Section Preservation.
          
   Lemma impe2_type_preservation
         (G: context) (d: loc_mode) (S: set condition) (H: set esc_hatch) (m0: mem2) :
-    forall pc md (U: set condition) c r m K G' K' U,
+    forall pc md c r m K G' K',
       context_wt G d ->
-      cconfig2_ok pc md G d m0 (c, r, m, K) G' K' U ->
+      cconfig2_ok pc md G d m0 (c, r, m, K) G' K'->
       forall mdmid cmid rmid mmid rmid' mmid' kmid' tmid rfin mfin kfin tfin,
         imm_premise
           (cstep2 mdmid d (cmid, rmid, mmid, K') (rmid', mmid', kmid') tmid)
           (cstep2 md d (c, r, m, K) (rfin, mfin, kfin) tfin) ->
-        (exists pcmid Gmid Gmid' Umid,
+        (exists pcmid Gmid Gmid',
           policy_le pc pcmid ->
-          Umid = [] \/ (forall i, In i U -> In i Umid) ->
-          cconfig2_ok pcmid mdmid Gmid d m0 (cmid, rmid, mmid, K') Gmid' K' Umid).
+          cconfig2_ok pcmid mdmid Gmid d m0 (cmid, rmid, mmid, K') Gmid' K').
   Proof.
   Admitted.
  
@@ -528,34 +510,31 @@ End Adequacy.
 (***********************************)
 
 Section Guarantees.
-  Definition corresponds (G: context) (g: sec_spec) : Prop :=
-    (forall l p bt rt, g l = p -> (loc_context G) l = Some (Typ bt p, rt))
+  Definition corresponds (G: context) : Prop :=
+    (forall l p bt rt, g0 l = p -> (loc_context G) l = Some (Typ bt p, rt))
     /\ (forall x, (var_context G) x = Some (Typ Tnat (LevelP L))).
   
   Lemma obs_equal (m1 m2: mem) (c: com) (tobs: trace) (t: trace2) :
-    forall pc md G d m0 r k G' r' m' k' m U,
+    forall pc md G d m0 r k G' r' m' k' m,
       merge_mem m1 m2 m ->
-      cconfig2_ok pc md G d m0 (c,r,m,k) G' k' U ->
+      cconfig2_ok pc md G d m0 (c,r,m,k) G' k' ->
       cstep2 md d (c,r,m,k) (r',m',k') t ->
       tobs = project_trace t true ->
       tobs_sec_level L tobs = tobs_sec_level L (project_trace t false).
   Proof.
   Admitted.
 
-  Lemma cstep_deterministic (c: com) (t1 t2: trace2) :
-    forall md d r m k r' m' k' r'' m'' k'',
-    cstep2 md d (c,r,m,k) (r',m',k') t1 ->
-    cstep2 md d (c,r,m,k) (r'',m'',k'') t2 ->
-    t1 = t2 /\ r'=r'' /\ m' = m'' /\ k'=k''.
+  Lemma com_type_k'_implies_cstep2_k' (c: com) : forall G G' K' md d r m k r' m' k' t,
+    com_type (LevelP L) Normal G nil nil d c G' K' ->
+    cstep2 md d (c,r,m,k) (r',m',KSingle k') t ->
+    k' = K'.
   Proof.
   Admitted.
-
-  (*Lemma U_only_shrinks : *)
-  (* XXX some weird stuff with U going on *)
-  Lemma diff_loc_protected_SC : forall m0 g U mknown l,
-      knowledge_ind m0 g U L mknown ->
+      
+  Lemma diff_loc_protected : forall m0 mknown l,
+      knowledge_ind m0 L mknown ->
       m0 l <> mknown l ->
-      protected (g l) SC.
+      protected (g0 l).
   Proof.
   Admitted.
 
@@ -565,39 +544,38 @@ Section Guarantees.
   Proof.
   Admitted.
   
-  (* ensure that conditions never unset in trace *)
-  Lemma secure_passive : forall g G G' K' d c,
-    well_formed_spec g ->
-    corresponds G g ->
+  Lemma secure_passive : forall G G' K' d c,
+    well_formed_spec g0 ->
+    corresponds G ->
     context_wt G d ->
     com_type (LevelP L) Normal G nil nil d c G' K' ->
-    secure_prog L d g c.
+    secure_prog L d c.
   Proof.
     unfold secure_prog; intros.
     apply (obs_equal m0 mknown c tobs t (LevelP L) Normal G d
-                     m reg_init2 (KSingle []) G' r' m' (KSingle K') m []); auto.
+                     m reg_init2 (KSingle []) G' r' m' (KSingle K') m); auto.
     unfold cconfig2_ok; split; unfold_cfgs.
-    - intros. apply in_nil in H9. omega.
-    - split; intros. unfold project_kill; auto.
-      split; intros; destruct_pairs.
+    - intros. unfold project_kill; auto.
+    - split; intros; destruct_pairs.
       inversion H9.
       split; intros; destruct_pairs.
-      destruct H6. destruct H6. assert (In (Mem x) tobs). rewrite H6. apply in_eq.
-      apply (H7 x []) in H11.
       unfold corresponds in H0; destruct_pairs.
       unfold well_formed_spec in H.
       pose (H (Not_cnd l)) as Hgwf; destruct Hgwf; destruct_pairs.
-      pose H13 as Hg0.
-      apply (H0 (Not_cnd l) x1 bt rt) in Hg0.
+      pose H12 as Hg0.
+      apply (H0 (Not_cnd l) x bt rt) in Hg0.
       rewrite H10 in Hg0. inversion Hg0; subst.
-      apply (diff_loc_protected_SC m0 g0 [] mknown (Not_cnd l)); auto.
+      apply (diff_loc_protected m0 mknown (Not_cnd l)); auto.
       apply (vpair_iff_diff m0 mknown m v1 v2 (Not_cnd l)) in H3.
       apply H3 in H9; auto.
-      admit. (* XXX More mess with conditions and U *)
-      split; intros. unfold is_esc_hatch in H9; destruct_pairs
-      
-
-  Admitted.
+      split; intros; [ | split; intros]; auto.
+      apply project_merge_inv_mem in H3; destruct_pairs; subst; auto.
+    - assert (k' = K'). apply (com_type_k'_implies_cstep2_k'
+                                 c G G' K' Normal d reg_init2 m
+                                 (KSingle []) r' m' k' t); auto.
+      rewrite <- H9; auto.
+  Qed.
+  
 (*
   Definition g_prime (d: loc_mode) (g: sec_spec) (I: set enclave) : sec_spec :=
     fun l => match (d l) with
